Front.v
@@ -1,0 +1,79 @@
+Require Import Nat.
+Require Import Bool.
+Require Import Arith.
+Require Import Arith.Compare.
+
+From CritBit Require Import KeyUtil.
+From CritBit Require Import PrefixCritical.
+From CritBit Require Import SeqAccess.
+
+(* a CBT (non-empty) *)
+Inductive CBT {X : Type} : Type :=
+  | Leaf (k : list bool) (v : X)
+  | Branch (i : nat) (l r : CBT).
+
+(* precond: one-terminated k *)
+(* precond: t is a valid tree w.r.t. CBT_valid *)
+Fixpoint lookup {X : Type} (k : list bool) (t : CBT) : option X :=
+  match t with
+  | Leaf k' v => if key_eqb k k' then Some v else None
+  | Branch i l r => if ith_zer i k then lookup k r else lookup k l
+  end.
+
+Fixpoint find_best_key {X : Type} (k : list bool) (t : @CBT X) : (list bool) :=
+  match t with
+  | Leaf k' _ => k'
+  | Branch i l r => find_best_key k (if ith_zer i k then r else l)
+  end.
+
+Definition seed_CBT {X : Type} (k : list bool) (v : X) : CBT :=
+  Leaf k v.
+
+Definition is_beforeb (pos : option nat) (bound : nat) : bool :=
+  match pos with
+  | None => false
+  | Some i => i <? bound
+  end.
+
+Definition insert_as_branch {X : Type} (k : list bool) (v : X) (i : nat) (t : CBT) : CBT :=
+  if ith_zer i k then Branch i t (Leaf k v) else Branch i (Leaf k v) t.
+
+(* precond: t is a valid tree w.r.t. CBT_valid *)
+(* precond: i is the critical bit of k w.r.t. t *)
+Fixpoint insert_at {X : Type} (k : list bool) (v : X) (i : option nat) (t : CBT) : CBT :=
+  match t with
+  | Leaf k' v' =>  match i with
+                   | None => Leaf k v
+                   | Some cbit => insert_as_branch k v cbit t
+                   end
+  | Branch j l r => if is_beforeb i j
+      then match i with
+           | None => Leaf k v (* shoud never happen *)
+           | Some cbit => insert_as_branch k v cbit t
+           end
+      else (if ith_zer j k
+            then Branch j l (insert_at k v i r)
+            else Branch j (insert_at k v i l) r)
+  end.
+
+Definition critical_bit_CBT {X : Type} (k : list bool) (t : @CBT X) : option nat :=
+  critical_bit_zer k (find_best_key k t).
+
+
+(* precond: one-terminated k *)
+Definition insert {X : Type} (k : list bool) (v : X) (t : CBT) : CBT :=
+  insert_at k v (critical_bit_CBT k t) t.
+
+
+Definition empty_map {X : Type} (k : list bool) :=
+  @None X.
+
+Definition insert_map
+  {X : Type} (k : list bool) (v : X) (m : (list bool) -> option X) (k' : list bool) :=
+  if key_eqb k' k then Some v else m k'.
+
+Definition content {X : Type} (t : CBT) (k : list bool) := @lookup X k t.
+
+(* only the results on valid keys (i.e., one-terminated) are relevant for content equality *)
+Definition equal_content {X : Type} (c1 c2 : (list bool) -> option X) : Prop :=
+  forall k, (OneTerminated k) -> c1 k = c2 k.
